src/BoundedArithmetic/Interface.v
@@ -3,100 +3,244 @@ Require Import Coq.ZArith.ZArith.
 Require Import Crypto.Util.ZUtil.
 Require Import Crypto.Util.Notations.
 
-Local Open Scope nat_scope.
 Local Open Scope Z_scope.
 Local Open Scope type_scope.
 
-Definition size := nat.
+Create HintDb push_decode discriminated.
+Create HintDb pull_decode discriminated.
+Hint Extern 1 => progress autorewrite with push_decode in * : push_decode.
+Hint Extern 1 => progress autorewrite with pull_decode in * : pull_decode.
 
-Local Coercion Z.of_nat : nat >-> Z.
+Class decoder (n : Z) W :=
+  { decode : W -> Z }.
+Coercion decode : decoder >-> Funclass.
+Global Arguments decode {n W _} _.
+
+Class is_decode {n W} (decode : decoder n W) :=
+  decode_range : forall x, 0 <= decode x < 2^n.
 
 Section InstructionGallery.
-  Context (n:Z) (* bit-width of width of W *)
-          {W : Type}(* previously [BoundedType], [W] for word *)
-          (decode : W -> Z).
+  Context (n : Z) (* bit-width of width of [W] *)
+          {W : Type} (* bounded type, [W] for word *)
+          (Wdecoder : decoder n W).
   Local Notation imm := Z (only parsing). (* immediate (compile-time) argument *)
 
-  Class is_load_immediate (ldi:imm->W) :=
+  Record load_immediate := { ldi :> imm -> W }.
+
+  Class is_load_immediate {ldi : load_immediate}  :=
     decode_load_immediate : forall x, 0 <= x < 2^n -> decode (ldi x) = x.
 
-  Class is_shift_right_doubleword_immediate (shrd:W->W->imm->W) :=
+  Record shift_right_doubleword_immediate := { shrd :> W -> W -> imm -> W }.
+
+  Class is_shift_right_doubleword_immediate (shrd : shift_right_doubleword_immediate) :=
     decode_shift_right_doubleword :
       forall high low count,
         0 <= count < n
         -> decode (shrd high low count) = (((decode high << n) + decode low) >> count) mod 2^n.
 
-  Class is_shift_left_immediate (shl:W->imm->W) :=
+  Record shift_left_immediate := { shl :> W -> imm -> W }.
+
+  Class is_shift_left_immediate (shl : shift_left_immediate) :=
     decode_shift_left_immediate :
       forall r count, 0 <= count < n -> decode (shl r count) = (decode r << count) mod 2^n.
 
-  Class is_spread_left_immediate (sprl:W->imm->W*W(*high, low*)) :=
+  Record spread_left_immediate := { sprl :> W -> imm -> W * W (* [(high, low)] *) }.
+
+  Class is_spread_left_immediate (sprl : spread_left_immediate) :=
     {
-      fst_spread_left_immediate : forall r count, 0 <= count < n ->
-        decode (fst (sprl r count)) = (decode r << count) >> n;
-      snd_spread_left_immediate : forall r count, 0 <= count < n ->
-          decode (snd (sprl r count)) = (decode r << count) mod 2^n
+      decode_fst_spread_left_immediate : forall r count,
+        0 <= count < n
+        -> decode (fst (sprl r count)) = (decode r << count) >> n;
+      decode_snd_spread_left_immediate : forall r count,
+          0 <= count < n
+          -> decode (snd (sprl r count)) = (decode r << count) mod 2^n
     }.
 
-  Class is_mask_keep_low (mkl:W->imm->W) :=
+  Record mask_keep_low := { mkl :> W -> imm -> W }.
+
+  Class is_mask_keep_low (mkl : mask_keep_low) :=
     decode_mask_keep_low : forall r count,
       0 <= count < n -> decode (mkl r count) = decode r mod 2^count.
 
   Local Notation bit b := (if b then 1 else 0).
-  Class is_add_with_carry (adc:W->W->bool->bool*W) :=
+
+  Record add_with_carry := { adc :> W -> W -> bool -> bool * W }.
+
+  Class is_add_with_carry (adc : add_with_carry) :=
     {
-      fst_add_with_carry : forall x y c, bit (fst (adc x y c)) = (decode x + decode y + bit c) >> n;
-      snd_add_with_carry : forall x y c, decode (snd (adc x y c)) = (decode x + decode y + bit c) mod (2^n)
+      bit_fst_add_with_carry : forall x y c, bit (fst (adc x y c)) = (decode x + decode y + bit c) >> n;
+      decode_snd_add_with_carry : forall x y c, decode (snd (adc x y c)) = (decode x + decode y + bit c) mod (2^n)
     }.
+
+  Record sub_with_carry := { subc :> W -> W -> bool -> bool * W }.
 
   Class is_sub_with_carry (subc:W->W->bool->bool*W) :=
     {
-    fst_sub_with_carry : forall x y c, fst (subc x y c) = ((decode x - decode y - bit c) <? 0);
-    snd_sub_with_carry : forall x y c, decode (snd (subc x y c)) = (decode x - decode y - bit c) mod 2^n
+      fst_sub_with_carry : forall x y c, fst (subc x y c) = ((decode x - decode y - bit c) <? 0);
+      decode_snd_sub_with_carry : forall x y c, decode (snd (subc x y c)) = (decode x - decode y - bit c) mod 2^n
     }.
 
-  Class is_mul (mul:W->W->W) :=
-    decode_mul : forall x y, decode (mul x y) = decode x * decode y mod 2^n.
+  Record multiply := { mul :> W -> W -> W }.
 
-  Class is_mul_low_low (w:Z) (mulhwll:W->W->W) :=
+  Class is_mul (mul : multiply) :=
+    decode_mul : forall x y, decode (mul x y) = (decode x * decode y) mod 2^n.
+
+  Record multiply_low_low := { mulhwll :> W -> W -> W }.
+  Record multiply_high_low := { mulhwhl :> W -> W -> W }.
+  Record multiply_high_high := { mulhwhh :> W -> W -> W }.
+
+  Class is_mul_low_low (w:Z) (mulhwll : multiply_low_low) :=
     decode_mul_low_low :
       forall x y, decode (mulhwll x y) = ((decode x mod 2^w) * (decode y mod 2^w)) mod 2^n.
-  Class is_mul_high_low (w:Z) (mulhwhl:W->W->W) :=
+  Class is_mul_high_low (w:Z) (mulhwhl : multiply_high_low) :=
     decode_mul_high_low :
       forall x y, decode (mulhwhl x y) = ((decode x >> w) * (decode y mod 2^w)) mod 2^n.
-  Class is_mul_high_high (w:Z) (mulhwhh:W->W->W) :=
+  Class is_mul_high_high (w:Z) (mulhwhh : multiply_high_high) :=
     decode_mul_high_high :
       forall x y, decode (mulhwhh x y) = ((decode x >> w) * (decode y >> w)) mod 2^n.
+
+  Record select_conditional := { selc :> bool -> W -> W -> W }.
+
+  Class is_select_conditional (selc : select_conditional) :=
+    decode_select_conditional : forall b x y,
+      decode (selc b x y) = if b then decode x else decode y.
+
+  Record add_modulo := { addm :> W -> W -> W (* modulus *) -> W }.
+
+  Class is_add_modulo (addm : add_modulo) :=
+    decode_add_modulo : forall x y modulus,
+      decode (addm x y modulus) = (decode x + decode y) mod (decode modulus).
 End InstructionGallery.
+
+Global Arguments load_immediate : clear implicits.
+Global Arguments shift_right_doubleword_immediate : clear implicits.
+Global Arguments shift_left_immediate : clear implicits.
+Global Arguments spread_left_immediate : clear implicits.
+Global Arguments mask_keep_low : clear implicits.
+Global Arguments add_with_carry : clear implicits.
+Global Arguments sub_with_carry : clear implicits.
+Global Arguments multiply : clear implicits.
+Global Arguments multiply_low_low : clear implicits.
+Global Arguments multiply_high_low : clear implicits.
+Global Arguments multiply_high_high : clear implicits.
+Global Arguments select_conditional : clear implicits.
+Global Arguments add_modulo : clear implicits.
+Global Arguments ldi {_ _} _.
+Global Arguments shrd {_ _} _ _ _.
+Global Arguments shl {_ _} _ _.
+Global Arguments sprl {_ _} _ _.
+Global Arguments mkl {_ _} _ _.
+Global Arguments adc {_ _} _ _ _.
+Global Arguments subc {_ _} _ _ _.
+Global Arguments mul {_ _} _ _.
+Global Arguments mulhwll {_ _} _ _.
+Global Arguments mulhwhl {_ _} _ _.
+Global Arguments mulhwhh {_ _} _ _.
+Global Arguments selc {_ _} _ _ _.
+Global Arguments addm {_ _} _ _ _.
+
+Existing Class load_immediate.
+Existing Class shift_right_doubleword_immediate.
+Existing Class shift_left_immediate.
+Existing Class spread_left_immediate.
+Existing Class mask_keep_low.
+Existing Class add_with_carry.
+Existing Class sub_with_carry.
+Existing Class multiply.
+Existing Class multiply_low_low.
+Existing Class multiply_high_low.
+Existing Class multiply_high_high.
+Existing Class select_conditional.
+Existing Class add_modulo.
+
+Global Arguments is_decode {_ _} _.
+Global Arguments is_load_immediate {_ _ _} _.
+Global Arguments is_shift_right_doubleword_immediate {_ _ _} _.
+Global Arguments is_shift_left_immediate {_ _ _} _.
+Global Arguments is_spread_left_immediate {_ _ _} _.
+Global Arguments is_mask_keep_low {_ _ _} _.
+Global Arguments is_add_with_carry {_ _ _} _.
+Global Arguments is_sub_with_carry {_ _ _} _.
+Global Arguments is_mul {_ _ _} _.
+Global Arguments is_mul_low_low {_ _ _} _ _.
+Global Arguments is_mul_high_low {_ _ _} _ _.
+Global Arguments is_mul_high_high {_ _ _} _ _.
+Global Arguments is_select_conditional {_ _ _} _.
+Global Arguments is_add_modulo {_ _ _} _.
+
+Ltac bounded_sovlver_tac :=
+  solve [ eassumption | typeclasses eauto | omega | auto 6 using decode_range with typeclass_instances omega ].
+
+Hint Rewrite @decode_load_immediate @decode_shift_right_doubleword @decode_shift_left_immediate @decode_fst_spread_left_immediate @decode_snd_spread_left_immediate @decode_mask_keep_low @bit_fst_add_with_carry @decode_snd_add_with_carry @fst_sub_with_carry @decode_snd_sub_with_carry @decode_mul @decode_mul_low_low @decode_mul_high_low @decode_mul_high_high @decode_select_conditional @decode_add_modulo using bounded_sovlver_tac : push_decode.
+
+Ltac push_decode :=
+  repeat first [ erewrite !decode_load_immediate by bounded_sovlver_tac
+               | erewrite !decode_shift_right_doubleword by bounded_sovlver_tac
+               | erewrite !decode_shift_left_immediate by bounded_sovlver_tac
+               | erewrite !decode_fst_spread_left_immediate by bounded_sovlver_tac
+               | erewrite !decode_snd_spread_left_immediate by bounded_sovlver_tac
+               | erewrite !decode_mask_keep_low by bounded_sovlver_tac
+               | erewrite !bit_fst_add_with_carry by bounded_sovlver_tac
+               | erewrite !decode_snd_add_with_carry by bounded_sovlver_tac
+               | erewrite !fst_sub_with_carry by bounded_sovlver_tac
+               | erewrite !decode_snd_sub_with_carry by bounded_sovlver_tac
+               | erewrite !decode_mul by bounded_sovlver_tac
+               | erewrite !decode_mul_low_low by bounded_sovlver_tac
+               | erewrite !decode_mul_high_low by bounded_sovlver_tac
+               | erewrite !decode_mul_high_high by bounded_sovlver_tac
+               | erewrite !decode_select_conditional by bounded_sovlver_tac
+               | erewrite !decode_add_modulo by bounded_sovlver_tac ].
+Ltac pull_decode :=
+  repeat first [ erewrite <- !decode_load_immediate by bounded_sovlver_tac
+               | erewrite <- !decode_shift_right_doubleword by bounded_sovlver_tac
+               | erewrite <- !decode_shift_left_immediate by bounded_sovlver_tac
+               | erewrite <- !decode_fst_spread_left_immediate by bounded_sovlver_tac
+               | erewrite <- !decode_snd_spread_left_immediate by bounded_sovlver_tac
+               | erewrite <- !decode_mask_keep_low by bounded_sovlver_tac
+               | erewrite <- !bit_fst_add_with_carry by bounded_sovlver_tac
+               | erewrite <- !decode_snd_add_with_carry by bounded_sovlver_tac
+               | erewrite <- !fst_sub_with_carry by bounded_sovlver_tac
+               | erewrite <- !decode_snd_sub_with_carry by bounded_sovlver_tac
+               | erewrite <- !decode_mul by bounded_sovlver_tac
+               | erewrite <- !decode_mul_low_low by bounded_sovlver_tac
+               | erewrite <- !decode_mul_high_low by bounded_sovlver_tac
+               | erewrite <- !decode_mul_high_high by bounded_sovlver_tac
+               | erewrite <- !decode_select_conditional by bounded_sovlver_tac
+               | erewrite <- !decode_add_modulo by bounded_sovlver_tac ].
 
 Module fancy_machine.
   Local Notation imm := Z (only parsing).
-  Class instructions (n:Z) :=
+
+  Class instructions (n : Z) :=
     {
       W : Type (* [n]-bit word *);
-      ldi : imm -> W;
-      shrd : W->W->imm -> W;
-      sprl : W->imm -> W*W;
-      mkl : W->imm -> W;
-      adc : W->W->bool -> bool*W;
-      subc : W->W->bool -> bool*W
+      decode :> decoder n W;
+      ldi :> load_immediate W;
+      shrd :> shift_right_doubleword_immediate W;
+      shl :> shift_left_immediate W;
+      mkl :> mask_keep_low W;
+      adc :> add_with_carry W;
+      subc :> sub_with_carry W;
+      mulhwll :> multiply_low_low W;
+      mulhwhl :> multiply_high_low W;
+      mulhwhh :> multiply_high_high W;
+      selc :> select_conditional W;
+      addm :> add_modulo W
     }.
 
-  Class arithmetic {n} (ops:instructions n) :=
+  Class arithmetic {n_over_two} (ops:instructions (2 * n_over_two)) :=
     {
-      decode : W -> Z;
-      decode_range : forall x, 0 <= decode x < 2^n;
-      load_immediate : is_load_immediate n decode ldi;
-      shift_right_doubleword_immediate : is_shift_right_doubleword_immediate n decode shrd;
-      spread_left_immediate : is_spread_left_immediate n decode sprl;
-      mask_keep_low : is_mask_keep_low n decode mkl;
-      add_with_carry : is_add_with_carry n decode adc;
-      sub_with_carry : is_sub_with_carry n decode subc
+      decode_range :> is_decode decode;
+      load_immediate :> is_load_immediate ldi;
+      shift_right_doubleword_immediate :> is_shift_right_doubleword_immediate shrd;
+      shift_left_immediate :> is_shift_left_immediate shl;
+      mask_keep_low :> is_mask_keep_low mkl;
+      add_with_carry :> is_add_with_carry adc;
+      sub_with_carry :> is_sub_with_carry subc;
+      multiply_low_low :> is_mul_low_low n_over_two mulhwll;
+      multiply_high_low :> is_mul_high_low n_over_two mulhwhl;
+      multiply_high_high :> is_mul_high_high n_over_two mulhwhh;
+      select_conditional :> is_select_conditional selc;
+      add_modulo :> is_add_modulo addm
     }.
-  Global Existing Instance load_immediate.
-  Global Existing Instance shift_right_doubleword_immediate.
-  Global Existing Instance spread_left_immediate.
-  Global Existing Instance mask_keep_low.
-  Global Existing Instance add_with_carry.
-  Global Existing Instance sub_with_carry.
 End fancy_machine.
